---
title: "Arithmetic Operators"
layout: "default"
---
The five arithmetic operators (`+`, `-`, `*`, `/`, `%`) are familiar to most people.

### Additive Operators
|Operator|Name   |
|:------:|:------|
|+       |Plus   |
|-       |Minus  |

The additive operators provide for basic addition and subtraction.

    assert 1 + 1 == 2
    assert 10 - 9 == 1
    
Additive operators are left-associative - they are assessed from left to right:
    
    assert 1 + 4 - 3 == 2

The `+` operator can also be used to concatenate two strings:

    String mySentence = 'This is a game ' + 'of two halves'

### Multiplicative Operators

|Operator|Name     |
|:------:|:--------|
|*       |Multiply |
|/       |Divide   |
|%       |Remainder|

The remainder operator (`%`) is also commonly referred to as the _modulus_ operator. The 

    assert 13 % 2 == 1

Multiplicative operators are left-associative:

    assert 10 * 6 / 2 == 30

### Precedence
Multiplicative operators have precedence over additive operators. 

    assert 10 - 1 * 10 == 0
    
If the result above is surprising and the expected result was 90 then parentheses "`()`" should have been used:

    assert (10 - 1) * 10 == 90
    
The elements within parentheses have precedence over the rest of the evaluation. This results in `(10 - 1)` being evaluated first and the result being multiplied by 10.

If we consider Pythagoras' theorem ($$$a^2 + b^2 = c^2$$$) the operator precedence will yield the correct answer without requiring parentheses:

    assert 3 * 3 + 4 * 4 == 5 * 5 
   
However, we could use parentheses purely for the sake of clarity:

    assert (3 * 3) + (4 * 4) == (5 * 5)
    
Nested parentheses can be used to further delineate an expression. The innermost parentheses are evaluated first, then moving outwards:

    assert ((10 - 1) * 10) / 2 == 45
    
In the equation above, `(10 - 1)` is evaluated first, the result (9) then being multiplied by 10 and that result (90) being divided by 2.

For significantly more complex calculations such as the quadratic equation (below) parentheses are required if the calculation is to be performed in a single expression:

$$x = {-b \pm \sqrt{b^2-4ac} \over 2a}$$

    def a = 5
    def b = 6
    def c = 1
    def x
    x = ((-1 * b) + Math.sqrt((b * b) - (4 * a * c))) / (2 * a)
    assert x == -0.2
    
_Note: The solution given above is not a complete implementation of the equation - it is provided for demonstration purposes ony._